
<rdf:RDF xmlns:rdf="http://www.w3.org/1999/02/22-rdf-syntax-ns#"
        xmlns:rdfs="http://www.w3.org/2000/01/rdf-schema#"
        xmlns:misc="http://xmlns.com/foaf/0.1/"
        xmlns:wot="http://xmlns.com/wot/0.1/"
        xmlns:wn="http://xmlns.com/wordnet/1.6/"
        xmlns:dc="http://purl.org/dc/elements/1.1/" >




<!-- 
classes:

-->

 <rdfs:Class
 rdf:about="http://xmlns.com/wot/0.1/PubKey"
 rdfs:label="Public Key"
 rdfs:comment="A class to represent a person's or organization's PGP
public key." />
 

 <rdfs:Class
 rdf:about="http://xmlns.com/wot/0.1/User"
 rdfs:label="PGP Key User"
 rdfs:comment="A wot subclass of foaf Person - the user of a PGP public
key">
 
  <rdfs:subClassOf rdf:resource="http://xmlns.com/foaf/0.1/Person" />

 </rdfs:Class> 

 <rdfs:Class
 rdf:about="http://xmlns.com/wot/0.1/SigEvent"
 rdfs:label="Signing Event"
 rdfs:comment="A PGP key signing event" >
 
<rdfs:subClassOf rdf:resource="http://xmlns.com/wordnet/1.6/Event"/>

 </rdfs:Class> 

 <rdfs:Class
 rdf:about="http://xmlns.com/wot/0.1/Endorsement"
 rdfs:label="Endorsement"
 rdfs:comment="An endorsement object, whose uri should be the location of an
ascii signature" >
 
<rdfs:subClassOf rdf:resource="http://xmlns.com/wordnet/1.6/Endorsement" />

 </rdfs:Class> 

<!--properties-->

 <rdf:Property rdf:about="http://xmlns.com/wot/0.1/hex_id" 

	rdfs:label="Public key hex identifier" 
	rdfs:comment="A public key hex identifier string">

	<rdfs:domain rdf:resource="http://xmlns.com/wot/0.1/PubKey" />
	<rdfs:range
rdf:resource="http://www.w3.org/2000/01/rdf-schema#Literal" />

 </rdf:Property>



 <rdf:Property rdf:about="http://xmlns.com/wot/0.1/length" 

	rdfs:label="Public Key length" 
	rdfs:comment="A string representing public key length">

	<rdfs:domain rdf:resource="http://xmlns.com/wot/0.1/PubKey" />
	<rdfs:range
rdf:resource="http://www.w3.org/2000/01/rdf-schema#Literal" />

 </rdf:Property>

 <rdf:Property rdf:about="http://xmlns.com/wot/0.1/fingerprint" 

	rdfs:label="Public Key Fingerprint" 
	rdfs:comment="A public key fingerprint string">

	<rdfs:domain rdf:resource="http://xmlns.com/wot/0.1/PubKey" />
	<rdfs:range
rdf:resource="http://www.w3.org/2000/01/rdf-schema#Literal" />

 </rdf:Property>


 <rdf:Property rdf:about="http://xmlns.com/wot/0.1/identity" 

	rdfs:label="identity" 
	rdfs:comment="A property linking to the User of the PGP key.">

	<rdfs:domain rdf:resource="http://xmlns.com/wot/0.1/PubKey" />
	<rdfs:range rdf:resource="http://xmlns.com/wot/0.1/User" />

 </rdf:Property>

 <rdf:Property rdf:about="http://xmlns.com/wot/0.1/signed" 

	rdfs:label="signed" 
	rdfs:comment="A property linking a public key to signature
events.">

	<rdfs:domain rdf:resource="http://xmlns.com/wot/0.1/User" />
	<rdfs:range rdf:resource="http://xmlns.com/wot/0.1/SigEvent" />

 </rdf:Property>

 <rdf:Property rdf:about="http://xmlns.com/wot/0.1/sigdate" 

	rdfs:label="signing date" 
	rdfs:comment="The date of a sining event.">
<!--also a time?-->

	<rdfs:domain rdf:resource="http://xmlns.com/wot/0.1/SigEvent" />
	<rdfs:range rdf:resource="http://www.w3.org/2000/01/rdf-schema#Literal" />

<!-- should be a datatype-->

 </rdf:Property>

 <rdf:Property rdf:about="http://xmlns.com/wot/0.1/signerLongHexID" 

	rdfs:label="signer long hex id" 
	rdfs:comment="The hex id of the signer's key">

	<rdfs:domain rdf:resource="http://xmlns.com/wot/0.1/SigEvent" />
	<rdfs:range rdf:resource="http://www.w3.org/2000/01/rdf-schema#Literal" />

 </rdf:Property>

 <rdf:Property rdf:about="http://xmlns.com/wot/0.1/pubkeyAddress" 

	rdfs:label="public key address" 
	rdfs:comment="The location of the public key used to sign the present document" >

	<rdfs:domain rdf:resource="http://www.w3.org/2000/01/rdf-schema#Resource" />
	<rdfs:range rdf:resource="http://www.w3.org/2000/01/rdf-schema#Resource" />

 </rdf:Property>

 <rdf:Property rdf:about="http://xmlns.com/wot/0.1/assurance" 

	rdfs:label="assurance" 
	rdfs:comment="Property pointing to an endorsment object which in
turn points to the location of the textual signature assuring the current
document" >

	<rdfs:domain rdf:resource="http://www.w3.org/2000/01/rdf-schema#Resource" />
	<rdfs:range rdf:resource="http://xmlns.com/wot/0.1/Endorsement" />

 </rdf:Property>




</rdf:RDF>


